lemma for value analysis

backend/Constprop.v
@@ -255,3 +255,386 @@ Definition transf_fundef (rm: romem) (fd: fundef) : fundef :=
 Definition transf_program (p: program) : program :=
   let rm := romem_for p in
   transform_program (transf_fundef rm) p.
+
+
+(** *Abstract Value Alpha Renaming *)
+
+Definition alpha_rename_aptr (a:permutation) (p:aptr) :=
+  match p with
+  | Gl id ofs => Gl (alpha_rename a id) ofs
+  | Glo id => Glo (alpha_rename a id)
+  | _ => p
+  end.
+
+Program Instance Alpha_aptr: Alpha aptr :=
+  { alpha_rename := alpha_rename_aptr }.
+Next Obligation.
+  destruct p;simpl;auto.
+Defined.
+Next Obligation.
+  destruct p1;auto;simpl;
+  erewrite alpha_rename_sym;auto.
+Defined.
+Next Obligation.
+  destruct p1;auto.
+Defined.
+
+Global Opaque Alpha_aptr.
+
+Definition alpha_rename_aval (a:permutation) (v:aval) :=
+  match v with
+  | Uns p n => Uns (alpha_rename a p) n
+  | Sgn p n => Sgn (alpha_rename a p) n
+  | Ptr p => Ptr (alpha_rename a p)
+  | Ifptr p => Ifptr (alpha_rename a p)
+  | _ => v
+  end.
+
+Program Instance Alpha_aval: Alpha aval :=
+  { alpha_rename := alpha_rename_aval }.
+Next Obligation.
+  destruct p;simpl;auto;
+  erewrite alpha_rename_refl;auto.
+Defined.
+Next Obligation.
+  destruct p1;auto;simpl;
+  erewrite alpha_rename_sym;auto.
+Defined.
+Next Obligation.
+  destruct p1;auto;simpl;
+  erewrite alpha_rename_trans;auto.
+Defined.
+
+Global Opaque Alpha_aval.
+
+Definition alpha_rename_acontent (a:permutation) (c:acontent) :=
+  match c with
+  | ACval chunk v => ACval chunk (alpha_rename a v)
+  end.
+
+Program Instance Alpha_acontent: Alpha acontent :=
+  { alpha_rename := alpha_rename_acontent }.
+Next Obligation.
+  destruct p;simpl;auto;
+  erewrite alpha_rename_refl;auto.
+Defined.
+Next Obligation.
+  destruct p1;auto;simpl;
+  erewrite alpha_rename_sym;auto.
+Defined.
+Next Obligation.
+  destruct p1;auto;simpl;
+  erewrite alpha_rename_trans;auto.
+Defined.
+
+Global Opaque Alpha_acontent.
+
+Inductive match_option_alpha {A:Type} {ALA:Alpha A} (a:permutation) :option A -> option A -> Prop :=  
+| match_none_alpha : match_option_alpha a None None
+| match_some_alpha : forall a1 a2, a1 = alpha_rename a a2 ->
+                              match_option_alpha a (Some a1) (Some a2).
+
+Definition match_ablock_alpha a b1 b2 :=
+  (forall n ,match_option_alpha a (ZTree.get n b1.(ab_contents)) (ZTree.get n b2.(ab_contents)))
+  /\ b1.(ab_summary) = alpha_rename a b2.(ab_summary).
+
+
+Inductive  match_option_ablock_alpha a  :option ablock -> option ablock -> Prop :=
+ |match_none_ablock_alpha: match_option_ablock_alpha a None None
+ |match_some_ablock_alpha : forall b1 b2,
+     match_ablock_alpha a b1 b2 ->
+    match_option_ablock_alpha a (Some b1) (Some b2).
+
+Definition  match_romem_alpha a (rm1 rm2: romem) :  Prop :=
+  forall pc,
+    match_option_ablock_alpha a (rm1 ! pc) (rm2 ! pc).
+
+  
+Lemma romem_for_alpha :forall a ctx,
+    match_romem_alpha a (romem_for (alpha_rename a ctx)) (romem_for ctx).
+  intros.
+  Admitted.
+
+Inductive  match_aenv_alpha (a:permutation) : aenv -> aenv -> Prop :=
+| match_aenv_Bot_alpha : match_aenv_alpha a AE.Bot AE.Bot
+| match_aenv_Top_except_alpha: forall pt1 pt2 pc,
+    match_option_alpha a (pt1 ! pc) (pt2 ! pc) ->
+    match_aenv_alpha a (AE.Top_except pt1) (AE.Top_except pt2).
+
+Definition match_amem_alpha (a:permutation) am1 am2 : Prop :=
+  match_ablock_alpha a am1.(am_stack) am2.(am_stack) /\
+  (forall id, match_option_ablock_alpha a (am1.(am_glob) ! id) (am2.(am_glob) ! (alpha_rename a id))) /\
+  am1.(am_nonstack) = alpha_rename a am2.(am_nonstack) /\
+  am1.(am_top) = alpha_rename a am2.(am_top).
+
+
+Inductive match_VA_alpha a : VA.t -> VA.t -> Prop :=
+| match_Bot_alpha : match_VA_alpha a VA.Bot VA.Bot
+| match_State_alpha : forall ae1 ae2 am1 am2, 
+    match_aenv_alpha a ae1 ae2 ->
+    match_amem_alpha a am1 am2 ->
+    match_VA_alpha a (VA.State ae1 am1) (VA.State ae2 am2).
+
+
+(* Inductive match_option_VA_alpha a : option VA.t -> option VA.t -> Prop := *)
+(* | match_none_VA_alpha : match_option_VA_alpha a None None *)
+(* | match_some_VA_alpha : forall va1 va2,  *)
+(*     match_VA_alpha a va1 va2 -> *)
+(*     match_option_VA_alpha a (Some va1) (Some va2). *)
+
+Lemma analyze_alpha: forall f a ctx pc,
+    match_VA_alpha a ((analyze (romem_for (alpha_rename a ctx)) (alpha_rename a f))!!pc) ((analyze (romem_for ctx) f)!!pc) .
+Admitted.
+
+Lemma match_aenv_alpha_areg : forall a ae1 ae2 r,
+        match_aenv_alpha a ae1 ae2 ->
+        areg ae1 r =  alpha_rename a (areg ae2 r).
+Admitted.
+
+
+Lemma match_aenv_alpha_aregs : forall a ae1 ae2 l,
+        match_aenv_alpha a ae1 ae2 ->
+        aregs ae1 l = map (alpha_rename a) (aregs ae2 l).
+Admitted.
+
+Lemma eval_static_operation_alpha: forall a op ae1 ae2 l,
+    match_aenv_alpha a ae1 ae2 ->
+    eval_static_operation (alpha_rename a op) (aregs ae1 l) =
+    alpha_rename a (eval_static_operation op (aregs ae2 l)).
+Admitted.
+
+Lemma eval_static_addressing_alpha: forall a addr ae1 ae2 l,
+    match_aenv_alpha a ae1 ae2 ->
+    eval_static_addressing (alpha_rename a addr) (aregs ae1 l) =
+    alpha_rename a (eval_static_addressing addr (aregs ae2 l)).
+Admitted.
+
+Lemma eval_static_condition_alpha: forall a c ae1 ae2 l,
+    match_aenv_alpha a ae1 ae2 ->
+    eval_static_condition c (aregs ae1 l) =
+    eval_static_condition c (aregs ae2 l).
+Admitted.
+
+Lemma const_for_result_alpha: forall a av,
+    match_option_alpha a (const_for_result (alpha_rename a av)) (const_for_result av).
+  Admitted.
+
+Lemma op_strength_reduction_alpha: forall a o o1 o2 l l1 l2 ae1 ae2,
+    match_aenv_alpha a ae1 ae2 ->
+    op_strength_reduction (alpha_rename a o) l (aregs ae1 l) = (o1,l1) ->
+    op_strength_reduction o l (aregs ae2 l) = (o2,l2) ->
+    o1 = alpha_rename a o2 /\ l1 = l2.
+Admitted.
+
+Lemma addr_strength_reduction_alpha: forall a addr addr1 addr2 l l1 l2 ae1 ae2,
+    match_aenv_alpha a ae1 ae2 ->
+    addr_strength_reduction (alpha_rename a addr) l (aregs ae1 l) = (addr1,l1) ->
+    addr_strength_reduction addr l (aregs ae2 l) = (addr2,l2) ->
+    addr1 = alpha_rename a addr2 /\ l1 = l2.
+Admitted.
+
+Lemma builtin_args_strength_reduction_alpha: forall a ae1 ae2 l,
+        match_aenv_alpha a ae1 ae2 ->
+        forall l1, (builtin_args_strength_reduction ae1 (map (alpha_rename a) l) l1) = (map (alpha_rename a) (builtin_args_strength_reduction ae2 l l1)) .
+Admitted.
+
+Lemma cond_strength_reduction_alpha: forall a c ae1 ae2 l,
+    match_aenv_alpha a ae1 ae2 ->
+    cond_strength_reduction c l (aregs ae1 l) =
+    cond_strength_reduction c l (aregs ae2 l).
+Admitted.
+
+
+ Lemma eval_static_builtin_function_alpha: forall a ae1 ae2 am1 am2 rm1 rm2 b l,
+            match_aenv_alpha a ae1 ae2 ->
+            match_amem_alpha a am1 am2 ->
+            match_romem_alpha a rm1 rm2 ->
+            match_option_alpha a (eval_static_builtin_function ae1 am1 rm1 b (map (alpha_rename a) l)) (eval_static_builtin_function ae2 am2 rm2 b l).
+Admitted.
+
+ Lemma debug_strength_reduction_alpha: forall a ae1 ae2 l,
+        match_aenv_alpha a ae1 ae2 ->
+        debug_strength_reduction ae1 (map (alpha_rename a) l) =
+        map (alpha_rename a) (debug_strength_reduction ae2 l).
+ Admitted.
+   
+ 
+Lemma AE_set_match_alpha : forall a r v ae1 ae2,
+            match_aenv_alpha a ae1 ae2 ->
+            match_aenv_alpha a (AE.set r (alpha_rename a v) ae1) (AE.set r v ae2). 
+Admitted.
+
+Lemma successor_alpha: forall a f ae1 ae2 pc,
+            match_aenv_alpha a ae1 ae2 ->
+            successor (alpha_rename a f) ae1 pc = successor f ae2 pc.
+Admitted.
+
+Lemma loadv_alpha: forall a chunk rm1 rm2 am1 am2 av1 av2,
+        match_romem_alpha a rm1 rm2 ->
+        match_amem_alpha a am1 am2 ->
+        av1 = alpha_rename a av2 ->
+        loadv chunk rm1 am1 av1 = alpha_rename a (loadv chunk rm2 am2 av2).
+Admitted.
+
+Lemma transf_instr_alpha_aux :forall f a ctx n i,
+    transf_instr (alpha_rename a f)
+    (analyze (romem_for (alpha_rename a ctx)) (alpha_rename a f))
+    (romem_for (alpha_rename a ctx)) n
+    (alpha_rename a i) =
+  alpha_rename a
+    (transf_instr f (analyze (romem_for ctx) f) 
+                  (romem_for ctx) n i).
+Proof.
+  intros.
+  Transparent Alpha_function Alpha_instruction. 
+  generalize (analyze_alpha f a ctx).
+  intros Match. generalize (Match n). intros Match_n.
+  unfold transf_instr.
+  destruct i;simpl.
+  (* Inop *)
+  - inversion Match_n;simpl;auto.
+  (* Iop *)
+  - inversion Match_n;simpl;auto.
+    + generalize (eval_static_operation_alpha a o ae1 ae2 l H1).
+      intros M_eval.
+      rewrite M_eval.
+      generalize (const_for_result_alpha a (eval_static_operation o (aregs ae2 l))). intros.
+      inversion H3.
+      * destruct (op_strength_reduction (alpha_rename a o) l (aregs ae1 l)) eqn: ?.
+        destruct (op_strength_reduction o l (aregs ae2 l)) eqn:?.
+        eapply (op_strength_reduction_alpha _ _ _ _ _ _ _ _ _ H1 Heqp) in Heqp0.
+        destruct Heqp0. subst.
+        generalize (AE_set_match_alpha a r (eval_static_operation o (aregs ae2 l)) ae1 ae2 H1). intros.
+        eapply successor_alpha in H4.
+        erewrite H4.
+        simpl. auto.
+      * generalize (AE_set_match_alpha a r (eval_static_operation o (aregs ae2 l)) ae1 ae2 H1). intros.
+        eapply successor_alpha in H7.
+        erewrite H7.
+        simpl. subst. auto.
+  - inversion Match_n;simpl;auto.
+    generalize (eval_static_addressing_alpha a a0 ae1 ae2 l H1).
+    intros.
+    generalize (romem_for_alpha a ctx). intros.
+    generalize (loadv_alpha _ m _ _ _ _ _ _ H4 H2 H3). intros.
+    generalize (const_for_result_alpha a (loadv m (romem_for ctx) am2
+                                                (eval_static_addressing a0 (aregs ae2 l)))). intros.
+    rewrite H5.                 (* careful *)
+    inversion H6.
+    + destruct (addr_strength_reduction (alpha_rename a a0) l (aregs ae1 l)) eqn: ?.
+      destruct (addr_strength_reduction a0 l (aregs ae2 l)) eqn:?.
+      eapply (addr_strength_reduction_alpha _ _ _ _ _ _ _ _ _ H1 Heqp) in Heqp0.
+      destruct Heqp0. subst.
+      simpl. auto.
+    + subst. simpl. auto.
+  (* Istore *)
+  - inversion Match_n;simpl;auto.
+    destruct (addr_strength_reduction (alpha_rename a a0) l (aregs ae1 l)) eqn: ?.
+      destruct (addr_strength_reduction a0 l (aregs ae2 l)) eqn:?.
+      eapply (addr_strength_reduction_alpha _ _ _ _ _ _ _ _ _ H1 Heqp) in Heqp0.
+      destruct Heqp0. subst.
+      simpl. auto.
+  (* Icall *)
+  - inversion Match_n;simpl;auto.
+    destruct s0;simpl;auto.
+    generalize (match_aenv_alpha_areg a ae1 ae2 r0 H1). intros.
+    rewrite H3. destruct (areg ae2 r0);simpl;auto.
+    destruct p;simpl;auto.
+    simpl.
+    Transparent Alpha_aval Alpha_aptr. simpl.
+    destruct (Ptrofs.eq ofs Ptrofs.zero);simpl;auto.
+  (* Itailcall *)
+  - inversion Match_n;simpl;auto.
+    destruct s0;simpl;auto.
+    generalize (match_aenv_alpha_areg a ae1 ae2 r H1). intros.
+    rewrite H3. destruct (areg ae2 r);simpl;auto.
+    destruct p;simpl;auto.
+    simpl.
+    Transparent Alpha_aval Alpha_aptr. simpl.
+    destruct (Ptrofs.eq ofs Ptrofs.zero);simpl;auto.
+  (* Ibuiltin *)
+  - inversion Match_n;simpl;auto.
+    generalize (builtin_args_strength_reduction_alpha _ _ _ l H1). intros.   
+    destruct e;simpl;auto;try erewrite H3;auto.
+    + destruct b;simpl;auto.
+      * destruct (lookup_builtin_function name sg);simpl;auto.
+        generalize (romem_for_alpha a ctx). intros.
+        generalize (eval_static_builtin_function_alpha _ _ _ _ _ _ _ b l H1 H2 H4). intros.
+        inversion H5;simpl;auto.
+        subst.
+        generalize (const_for_result_alpha a a2). intros.
+        inversion H8;simpl.
+        -- rewrite <- H10;simpl;auto.
+        -- rewrite <- H9;subst;auto.
+    + erewrite debug_strength_reduction_alpha;auto.
+  (* Icond *)
+  - inversion Match_n;simpl;auto.
+    erewrite (eval_static_condition_alpha _ _ _ _ _ H1).
+    destruct (resolve_branch (eval_static_condition c (aregs ae2 l)));simpl;auto.
+    destruct b;simpl;auto.
+    destruct (cond_strength_reduction c l (aregs ae1 l)) eqn: ?.
+    destruct (cond_strength_reduction c l (aregs ae2 l)) eqn:?.
+    apply (cond_strength_reduction_alpha _ c _ _ l) in H1;auto.
+    rewrite H1 in Heqp. rewrite Heqp in Heqp0. inversion Heqp0.
+    simpl. auto.
+  (* Ijumptable *)
+  - inversion Match_n;simpl;auto.
+    generalize (match_aenv_alpha_areg a ae1 ae2 r H1). intros.
+    rewrite H3. destruct (areg ae2 r);simpl;auto.
+    destruct (list_nth_z l (Int.unsigned n0));simpl;auto.
+  (* Ireturn *)
+  - inversion Match_n;simpl;auto.
+Qed.
+
+Lemma  transf_function_alpha_aux : forall f a ctx n,
+    PTree.xmap (transf_instr (alpha_rename a f)
+                             (analyze (romem_for (alpha_rename a ctx)) (alpha_rename a f))
+                             (romem_for (alpha_rename a ctx)))
+               (PTree.map1 (alpha_rename a) (fn_code f)) n =
+    PTree.map1 (alpha_rename a)
+               (PTree.xmap (transf_instr f (analyze (romem_for ctx) f) (romem_for ctx))
+                           (fn_code f) n).
+Proof.
+  intros. generalize dependent n.
+  induction (fn_code f);intros.
+  - simpl. auto.
+  - simpl.
+    destruct o;simpl.
+    + f_equal;auto.
+      f_equal. apply transf_instr_alpha_aux.
+    + f_equal;auto.
+Qed.
+
+
+(* final lemma *)
+
+Lemma transf_function_alpha: forall f a ctx,
+    transf_function (romem_for (alpha_rename a ctx)) (alpha_rename a f) =
+    alpha_rename a (transf_function (romem_for ctx) f).
+Proof.
+  Transparent Alpha_prog Alpha_function.
+  intros.
+  simpl.
+  unfold transf_function.
+  unfold alpha_rename_function.
+  f_equal.
+   assert ({|
+          fn_sig := fn_sig f;
+          fn_params := fn_params f;
+          fn_stacksize := fn_stacksize f;
+          fn_code := PTree.map1 (alpha_rename a) (fn_code f);
+          fn_entrypoint := fn_entrypoint f |} = alpha_rename a f).
+  { simpl. unfold alpha_rename_function. auto. }
+  rewrite H. clear H. simpl. 
+  unfold PTree.map.
+  apply transf_function_alpha_aux.
+Qed.
+
+Lemma transf_fundef_alpha: forall fd a ctx,
+    transf_fundef (romem_for (alpha_rename a ctx)) (alpha_rename a fd) = alpha_rename a (transf_fundef (romem_for ctx) fd).
+Proof.
+  intros.
+  Transparent Alpha_fundef.
+  destruct fd;simpl;auto.
+  f_equal. apply transf_function_alpha.
+Qed.
