backend/Renumberproof.v
@@ -261,10 +261,179 @@ Qed.
 
 End PRESERVATION.
 
-Instance TransfRenumberAlpha: TransfAlpha match_prog (@AST.prog_public _ _) (@AST.prog_public _ _).
-Admitted.
+(** *alpha and transf commute*)
+Lemma PTree_map_set {A B:Type}: forall b (k:positive) (v:A) (f:A->B),
+    PTree.map1 f (PTree.set k v b) = PTree.set k (f v) (PTree.map1 f b).
+Proof.
+  induction b.
+  - intros. simpl. induction k. 
+    + simpl. rewrite IHk. auto.
+    + simpl. rewrite IHk. auto.
+    + simpl.  auto.
+  - intros. simpl. induction k.
+    + simpl. rewrite IHb2. auto.
+    + simpl. rewrite IHb1. auto.
+    + simpl. auto.
+Qed.
+
+Lemma renum_instr_alpha_aux: forall permu f i,
+    AST.alpha_rename permu (renum_instr f i) =
+    renum_instr f (AST.alpha_rename permu i).
+Proof.
+  Transparent Alpha_instruction.
+  induction i;simpl;auto;
+    destruct s0;simpl;auto.
+Qed.
+
+Lemma renum_cfg_alpha_fold_left_aux: forall permu f fn_code b i,
+    PTree.map1 (AST.alpha_rename permu)
+               (fold_left (fun (a : code) (p : positive * instruction) =>
+                             renum_node f a (fst p) (snd p))
+                          (PTree.xelements fn_code i nil) b) =
+    fold_left
+      (fun (a : code) (p : positive * instruction) =>
+         renum_node f a (fst p) (snd p))
+      (PTree.xelements (PTree.map1 (AST.alpha_rename permu) fn_code) i
+                       nil) (PTree.map1 (AST.alpha_rename permu) b).
+Proof.
+  induction fn_code. 
+  - simpl. auto.
+  - simpl.
+    destruct o.
+    + simpl.
+      intros.
+      rewrite <- (app_nil_l ((PTree.prev i0, i) :: PTree.xelements fn_code2 i0~1 nil)).
+      rewrite <- (app_nil_l ((PTree.prev i0, alpha_rename_instruction permu i)
+        :: PTree.xelements
+             (PTree.map1 (alpha_rename_instruction permu) fn_code2)
+             i0~1 nil)).
+      rewrite PTree.xelements_append.
+      rewrite PTree.xelements_append.
+      rewrite fold_left_app. rewrite fold_left_app.
+      set (tf:=(fun (a : code) (p : positive * instruction) =>
+                  renum_node f a (fst p) (snd p))).
+      simpl.
+      erewrite IHfn_code2.
+      f_equal.
+      unfold tf. simpl.
+      unfold renum_node.
+      destruct (f ! (PTree.prev i0)).
+      * rewrite PTree_map_set. f_equal. 
+        apply renum_instr_alpha_aux. (* rename instruction *)
+        auto.
+      * auto.
+    + simpl.
+      intros.
+      rewrite <- (app_nil_l (PTree.xelements fn_code2 i~1 nil)).
+      rewrite <- (app_nil_l  (PTree.xelements
+          (PTree.map1 (alpha_rename_instruction permu) fn_code2) i~1
+          nil)).
+      rewrite PTree.xelements_append.
+      rewrite PTree.xelements_append.
+      rewrite fold_left_app. rewrite fold_left_app.
+      set (tf:=(fun (a : code) (p : positive * instruction) =>
+                  renum_node f a (fst p) (snd p))).
+      simpl.
+      erewrite IHfn_code2.
+      f_equal.
+      auto.
+Qed.
 
 
+Lemma renum_cfg_alpha_fold_aux : forall permu f fn_code b,
+    PTree.map1 (AST.alpha_rename permu)
+               (PTree.fold (renum_node f) fn_code b) =
+    PTree.fold (renum_node f)
+               (PTree.map1 (AST.alpha_rename permu) fn_code)
+               (PTree.map1  (AST.alpha_rename permu) b).
+Proof.
+  intros.
+  rewrite PTree.fold_spec.
+  rewrite PTree.fold_spec.
+  unfold PTree.elements.
+  apply renum_cfg_alpha_fold_left_aux.
+Qed.  
 
 
+Lemma renum_cfg_alpha_aux : forall permu f fn_code,
+  PTree.map1 (AST.alpha_rename permu) (renum_cfg f fn_code) =
+  renum_cfg f (PTree.map1 (AST.alpha_rename permu) fn_code).
+Proof.
+  unfold renum_cfg. intros.
+  apply renum_cfg_alpha_fold_aux.
+Qed.  
 
+Lemma alpha_transf_function_commute: forall f permu,
+    AST.alpha_rename permu (transf_function f) = transf_function (AST.alpha_rename permu f).
+Proof.
+  Transparent Alpha_function.
+  intros.
+  simpl. unfold transf_function.
+  destruct f. simpl.
+  unfold alpha_rename_function.
+  simpl.
+  unfold successors_map. simpl.
+  assert ((postorder (PTree.map1 successors_instr fn_code) fn_entrypoint) =  (postorder
+       (PTree.map1 successors_instr
+          (PTree.map1 (AST.alpha_rename permu) fn_code))
+       fn_entrypoint)).
+    {
+      f_equal.
+      induction fn_code.
+      simpl. auto.
+      simpl. rewrite IHfn_code1.
+      f_equal.
+      destruct o.
+      - simpl.
+        Transparent Alpha_instruction.
+        induction i;simpl;auto;
+          destruct s0;simpl;auto.
+      - simpl. auto.
+      - auto.
+    }
+  f_equal.
+  - rewrite -> H.
+    set (f:= (postorder (PTree.map1 successors_instr fn_code) fn_entrypoint)).
+    apply renum_cfg_alpha_fold_aux .
+    - f_equal. auto.
+Qed.
+    
+Lemma transf_fundef_alpha: forall fd permu,
+    transf_fundef (AST.alpha_rename permu fd) =
+    AST.alpha_rename permu (transf_fundef fd). 
+Proof.
+  Transparent AST.Alpha_fundef.
+  simpl.
+  intros.
+  destruct fd.
+  simpl.
+  f_equal. symmetry.
+  apply alpha_transf_function_commute.
+  simpl. auto.
+Qed.
+
+
+Instance TransfRenumberAlpha: TransfAlpha match_prog (fun p => p.(prog_main) :: p.(prog_public)) (fun p => p.(prog_main) :: p.(prog_public)).
+Proof.
+  red.
+  intros.
+  unfold match_prog in *.
+  unfold alpha_equiv in *. destruct H as [a [? ?]].
+  exists (alpha_rename a t).
+  split.
+  eapply alpha_program_match.
+  apply transf_fundef_alpha.
+
+  apply H0.
+  apply H1.
+  auto.
+  
+  exists a. split;auto.
+  generalize H0.
+  apply match_program_main in H0.
+  intros.
+  unfold match_program in H2.
+  apply match_program_public in H2. 
+  apply H. rewrite H0 in H3. rewrite H2 in H3.
+  auto.
+Qed.
